refine

proof/TypeClosedSimp.v
@@ -10,133 +10,226 @@ From PLF Require Import RfTypeDef.
 From PLF Require Import LinearContext.
 Import ListNotations.
 
-Definition ncontxt := linear_context ty.
+(* closed_refinement *)
+
+Definition state_order (st st': state) := (forall x c_x, st x = Some c_x -> st' x = Some c_x).
+Notation " st '<st<' st' " := (state_order st st') (at level 80).
+
+Lemma state_order_trans: forall st1 st2 st3, st1 <st< st2 -> st2 <st< st3 -> st1 <st< st3.
+Proof.
+  unfold state_order. intros. auto.
+Qed.
+
+Global Hint Resolve state_order_trans: core.
+
+Definition closed_refinement_under_state (st: state) (phi: refinement): Prop := forall st', st <st< st' -> phi st = phi st'.
+
+Global Hint Unfold closed_refinement_under_state: core.
+
+Definition empstate : state := empty.
+
+Lemma empstate_min: forall st, empstate <st< st.
+Proof.
+  intros. intros x c_x H. inversion H.
+Qed.
+
+Global Hint Resolve empstate_min: core.
+
+Lemma state_order_implies_closed: forall st st' phi,
+    st <st< st' -> closed_refinement_under_state st phi -> closed_refinement_under_state st' phi.
+Proof with eauto.
+  unfold closed_refinement_under_state. intros. rewrite <- H0...
+Qed.
+
+Global Hint Resolve state_order_implies_closed: core.
+
+Lemma constant_refinement_is_closed: forall (c: constant) (phi: refinement),
+    (forall st : state, phi st = (fun c' => c = c')) -> (closed_refinement_under_state empstate phi).
+Proof.
+  intros.
+  intros st HH. rewrite H. rewrite H. auto.
+Qed.
+
+Lemma refinement_subst_c_closed_rf: forall x1 c2 phi,
+    closed_refinement_under_state empstate phi -> refinement_subst_c x1 c2 phi = phi.
+Proof with eauto.
+  intros.
+  unfold closed_refinement_under_state in H. unfold refinement_subst_c.
+  apply functional_extensionality. intros st.
+  rewrite <- H...
+Qed.
+
+(* closed_type *)
+
+(* First we define the non-deter state *)
+
+Definition nstate := string -> option tm.
+
+Definition state_in_non_deter_state (st: state) (nst: nstate): Prop :=
+  forall x, (match nst x with
+        | None => True
+        | Some e =>
+            match st x with
+            | None => False
+            | Some c => e -->* c
+            end
+        end).
+
+Notation " st '\NSTin' nst " := (state_in_non_deter_state st nst) (at level 40).
+
+Definition phi_sat_nst (phi: refinement) (nst: nstate) (c: constant) :=
+  (forall st, st \NSTin nst -> closed_refinement_under_state st phi /\ phi st c).
+
+(* Global Hint Unfold nst_tmR_aux: core. *)
+
 Definition lcontxt := linear_context overunderty.
 
-Fixpoint ncontxt_to_basic_ctx_aux (Gamma: ncontxt) (ctx: partial_map ty) :=
-  match Gamma with
-  | nil => ctx
-  | (x, xty) :: Gamma => ncontxt_to_basic_ctx_aux Gamma (update ctx x xty)
-  end.
+Inductive closed_refinement_in_ctx : nstate -> lcontxt -> refinement -> Prop :=
+| closed_refinement_in_ctx_nil:
+  forall nst phi, (forall st, st \NSTin nst -> closed_refinement_under_state st phi) -> closed_refinement_in_ctx nst [] phi
+| closed_refinement_in_ctx_cons: forall nst x tau Gamma phi,
+    (forall (c_x: constant), empty |- c_x \Vin (ou\_ tau _/) ->
+                                closed_refinement_in_ctx (update nst x (tvalue c_x)) Gamma phi) ->
+    closed_refinement_in_ctx nst ((x, tau) :: Gamma) phi.
 
-Definition ncontxt_to_basic_ctx (Gamma: ncontxt) := ncontxt_to_basic_ctx_aux Gamma empty.
+Global Hint Constructors closed_refinement_in_ctx: core.
 
-Global Hint Unfold ncontxt_to_basic_ctx: core.
-
-Inductive type_closed_refinement : ncontxt -> base_ty -> refinement -> Prop :=
-| type_closed_refinement_nil: forall T phi, is_closed_refinement T phi -> type_closed_refinement [] T phi
-| type_closed_refinement_cons: forall x T Gamma Tphi phi,
-    (forall (c_x: constant), empty |- c_x \Vin T ->
-                                type_closed_refinement Gamma Tphi (fun st c => phi (t_update st x c_x) c)) ->
-    type_closed_refinement ((x, T) :: Gamma) Tphi phi.
-
-Global Hint Constructors type_closed_refinement: core.
-
-Lemma type_closed_refinement_weakening: forall Gamma1 Gamma2 Gamma3 T phi,
+Lemma closed_refinement_in_ctx_weakening: forall st Gamma1 Gamma2 Gamma3 phi,
     (Gamma1 ++ Gamma2) = Gamma3 ->
-    type_closed_refinement Gamma2 T phi ->
-    type_closed_refinement Gamma3 T phi.
+    closed_refinement_in_ctx st Gamma2 phi ->
+    closed_refinement_in_ctx st Gamma3 phi.
 Admitted.
 
-Module ExCloseRefinement.
+(* Module ExCloseRefinement. *)
 
-  Example true_refinement: is_closed_refinement TNat (fun _ c => c = 3).
-  Proof.
-    unfold is_closed_refinement. reflexivity.
-  Qed.
+(*   Example true_refinement: closed_refinement_under_state empsta (fun _ c => c = 3). *)
+(*   Proof. *)
+(*     unfold closed_refinement_under_state. reflexivity. *)
+(*   Qed. *)
 
-  (* When the type dismatch, it is equal to bottom refinement *)
-  Example true_refinement2: is_closed_refinement TNat (fun _ c => c = true).
-  Proof.
-    unfold is_closed_refinement. reflexivity.
-  Qed.
+(*   (* When the type dismatch, it is equal to bottom refinement *) *)
+(*   Example true_refinement2: closed_refinement_under_state TNat (fun _ c => c = true). *)
+(*   Proof. *)
+(*     unfold closed_refinement_under_state. reflexivity. *)
+(*   Qed. *)
 
-  Example refinement_under_nctx: type_closed_refinement [("x"%string, TBase TNat)] TNat (fun st c => c = st "x"%string).
-  Proof.
-    constructor. intros.
-    apply nat_value_n_exists in H. destruct H; subst.
-    constructor. constructor; subst; auto.
-  Qed.
+(*   Example refinement_under_nctx: closed_refinement_in_ctx [("x"%string, TBase TNat)] TNat (fun st c => c = st "x"%string). *)
+(*   Proof. *)
+(*     constructor. intros. *)
+(*     apply nat_value_n_exists in H. destruct H; subst. *)
+(*     constructor. constructor; subst; auto. *)
+(*   Qed. *)
 
-End ExCloseRefinement.
+(* End ExCloseRefinement. *)
 
-Inductive overunderbasety : Type :=
-| Obase: base_ty -> refinement -> overunderbasety
-| Ubase: base_ty -> refinement -> overunderbasety.
+Inductive st_type_closed_in_ctx : nstate -> lcontxt -> overunderty -> Prop :=
+| st_type_closed_base1: forall st Gamma (T: base_ty) phi,
+    closed_refinement_in_ctx st Gamma phi -> st_type_closed_in_ctx st Gamma ({{v: T | phi}})
+| st_type_closed_base2: forall st Gamma (T: base_ty) phi,
+    closed_refinement_in_ctx st Gamma phi -> st_type_closed_in_ctx st Gamma ([[v: T | phi]])
+| st_type_closed_oarr: forall st Gamma x T phi (tau: underty),
+    st_type_closed_in_ctx st Gamma ({{v: T | phi}}) ->
+    st_type_closed_in_ctx st ((x, Oty ({{v: T | phi}})) :: Gamma) tau ->
+    st_type_closed_in_ctx st Gamma (x o: ({{v: T | phi}}) o--> tau)
+| st_type_closed_arrarr: forall st Gamma (tau_x: underty) (tau: underty),
+    st_type_closed_in_ctx st Gamma tau_x ->
+    st_type_closed_in_ctx st Gamma tau ->
+    st_type_closed_in_ctx st Gamma (tau_x u--> tau).
 
-Definition basecontxt := linear_context overunderbasety.
+Global Hint Constructors st_type_closed_in_ctx: core.
 
-Fixpoint erase_basetypectx (Gamma: basecontxt): ncontxt :=
-  match Gamma with
-  | nil => nil
-  | (x, Obase T _)::Gamma => (x, TBase T)::(erase_basetypectx Gamma)
-  | (x, Ubase T _)::Gamma => (x, TBase T)::(erase_basetypectx Gamma)
-  end.
+Lemma st_type_closed_in_ctx_emp_implies_all_not_free: forall Gamma (tau: underty) x,
+    l_find_right_most Gamma x = None ->
+    st_type_closed_in_ctx empty Gamma tau ->
+    ~ appear_free_in_underty x tau.
+Admitted.
 
-Fixpoint erase_lctx (Gamma: lcontxt): ncontxt :=
-  match Gamma with
-  | nil => nil
-  | (x, tau)::Gamma => (x, ou\_ tau _/)::(erase_lctx Gamma)
-  end.
+Global Hint Resolve st_type_closed_in_ctx_emp_implies_all_not_free: core.
 
-Definition lctx_to_basic_ctx (Gamma: lcontxt) := ncontxt_to_basic_ctx_aux (erase_lctx Gamma) empty.
+Lemma st_type_closed_in_ctx_emp_implies_all: forall st Gamma tau,
+    st_type_closed_in_ctx empty Gamma tau -> st_type_closed_in_ctx st Gamma tau.
+Admitted.
 
-Global Hint Unfold lctx_to_basic_ctx: core.
+Global Hint Resolve st_type_closed_in_ctx_emp_implies_all: core.
 
-Inductive type_closed_in_basectx : basecontxt -> overunderty -> Prop :=
-| type_closed_base1: forall Gamma (T: base_ty) phi,
-    type_closed_refinement (erase_basetypectx Gamma) T phi ->
-    type_closed_in_basectx Gamma ({{v: T | phi}})
-| type_closed_base2: forall Gamma (T: base_ty) phi,
-    type_closed_refinement (erase_basetypectx Gamma) T phi ->
-    type_closed_in_basectx Gamma ([[v: T | phi]])
-| type_closed_oarr: forall Gamma x T phi (tau: underty),
-    type_closed_in_basectx Gamma ({{v: T | phi}}) ->
-    type_closed_in_basectx ((x, Obase T phi) :: Gamma) tau ->
-    type_closed_in_basectx Gamma (x o: ({{v: T | phi}}) o--> tau)
-| type_closed_arrarr: forall Gamma (tau_x: underty) (tau: underty),
-    type_closed_in_basectx Gamma tau_x ->
-    type_closed_in_basectx Gamma tau ->
-    type_closed_in_basectx Gamma (tau_x u--> tau).
+(* Inductive overunderbasety : Type := *)
+(* | Obase: base_ty -> refinement -> overunderbasety *)
+(* | Ubase: base_ty -> refinement -> overunderbasety. *)
 
-Global Hint Constructors type_closed_in_basectx: core.
+(* Definition basecontxt := linear_context overunderbasety. *)
+
+(* Fixpoint erase_basetypectx (Gamma: basecontxt): ncontxt := *)
+(*   match Gamma with *)
+(*   | nil => nil *)
+(*   | (x, Obase T _)::Gamma => (x, TBase T)::(erase_basetypectx Gamma) *)
+(*   | (x, Ubase T _)::Gamma => (x, TBase T)::(erase_basetypectx Gamma) *)
+(*   end. *)
+
+(* Fixpoint erase_lctx (Gamma: lcontxt): ncontxt := *)
+(*   match Gamma with *)
+(*   | nil => nil *)
+(*   | (x, tau)::Gamma => (x, ou\_ tau _/)::(erase_lctx Gamma) *)
+(*   end. *)
+
+(* Definition lctx_to_basic_ctx (Gamma: lcontxt) := ncontxt_to_basic_ctx_aux (erase_lctx Gamma) empty. *)
+
+(* Global Hint Unfold lctx_to_basic_ctx: core. *)
+
+(* Inductive type_closed_in_ctx : basecontxt -> overunderty -> Prop := *)
+(* | type_closed_base1: forall Gamma (T: base_ty) phi, *)
+(*     closed_refinement_in_ctx (erase_basetypectx Gamma) T phi -> *)
+(*     type_closed_in_ctx Gamma ({{v: T | phi}}) *)
+(* | type_closed_base2: forall Gamma (T: base_ty) phi, *)
+(*     closed_refinement_in_ctx (erase_basetypectx Gamma) T phi -> *)
+(*     type_closed_in_ctx Gamma ([[v: T | phi]]) *)
+(* | type_closed_oarr: forall Gamma x T phi (tau: underty), *)
+(*     type_closed_in_ctx Gamma ({{v: T | phi}}) -> *)
+(*     type_closed_in_ctx ((x, Obase T phi) :: Gamma) tau -> *)
+(*     type_closed_in_ctx Gamma (x o: ({{v: T | phi}}) o--> tau) *)
+(* | type_closed_arrarr: forall Gamma (tau_x: underty) (tau: underty), *)
+(*     type_closed_in_ctx Gamma tau_x -> *)
+(*     type_closed_in_ctx Gamma tau -> *)
+(*     type_closed_in_ctx Gamma (tau_x u--> tau). *)
 
 (* before erase refinement from the context, we will erase all function type bindings *)
-Fixpoint lcontxt_to_baseconctx (Gamma: lcontxt): basecontxt :=
-  match Gamma with
-  | nil => nil
-  | (x, ty)::Gamma =>
-      match ty with
-      | Oty ({{v: T | phi }}) => (x, Obase T phi)::(lcontxt_to_baseconctx Gamma)
-      | Uty ([[v: T | phi ]]) => (x, Ubase T phi)::(lcontxt_to_baseconctx Gamma)
-      | _ => (lcontxt_to_baseconctx Gamma)
-      end
-  end.
+(* Fixpoint lcontxt_to_baseconctx (Gamma: lcontxt): basecontxt := *)
+(*   match Gamma with *)
+(*   | nil => nil *)
+(*   | (x, ty)::Gamma => *)
+(*       match ty with *)
+(*       | Oty ({{v: T | phi }}) => (x, Obase T phi)::(lcontxt_to_baseconctx Gamma) *)
+(*       | Uty ([[v: T | phi ]]) => (x, Ubase T phi)::(lcontxt_to_baseconctx Gamma) *)
+(*       | _ => (lcontxt_to_baseconctx Gamma) *)
+(*       end *)
+(*   end. *)
 
-Definition type_closed (Gamma: lcontxt) (tau: overunderty):=
-  type_closed_in_basectx (lcontxt_to_baseconctx Gamma) tau.
+Definition type_closed_in_ctx (Gamma: lcontxt) (tau: overunderty):= st_type_closed_in_ctx empty Gamma tau.
 
-Global Hint Unfold type_closed: core.
+Global Hint Unfold type_closed_in_ctx: core.
 
 (* type closed \S{Ty} *)
 
-Lemma mk_op_is_type_closed: forall op a b, type_closed l_empty (mk_op op a b).
+Lemma mk_op_is_type_closed: forall op a b, type_closed_in_ctx l_empty (mk_op op a b).
 Admitted.
 
 Global Hint Resolve mk_op_is_type_closed: core.
 
-Lemma mk_eq_over_base_is_type_closed: forall x T phi, type_closed ((x, Oty ({{v:T | phi}}))::nil) (mk_eq_var T x).
+Lemma mk_eq_over_base_is_type_closed: forall x T phi, type_closed_in_ctx ((x, Oty ({{v:T | phi}}))::nil) (mk_eq_var T x).
 Proof with eauto.
   intros x T phi. repeat constructor...
-  unfold is_closed_refinement... intros st st'. rewrite t_update_eq. rewrite t_update_eq. reflexivity.
+  unfold closed_refinement_under_state... intros st Hst st' Hsub.
+  remember (Hst x) as Hst'. clear HeqHst'. rewrite update_eq in Hst'.
+  destruct (st x) eqn: HH... rewrite Hsub with (c_x := c)... inversion Hst'.
 Qed.
 
 Global Hint Resolve mk_eq_over_base_is_type_closed: core.
 
-Lemma mk_eq_under_base_is_type_closed: forall x T phi, type_closed ((x, Uty ([[v:T | phi]]))::nil) (mk_eq_var T x).
+Lemma mk_eq_under_base_is_type_closed: forall x T phi, type_closed_in_ctx ((x, Uty ([[v:T | phi]]))::nil) (mk_eq_var T x).
 Proof with eauto.
   intros x T phi. repeat constructor...
-  unfold is_closed_refinement... intros st st'. rewrite t_update_eq. rewrite t_update_eq. reflexivity.
+  unfold closed_refinement_under_state... intros st Hst st' Hsub.
+  remember (Hst x) as Hst'. clear HeqHst'. rewrite update_eq in Hst'.
+  destruct (st x) eqn: HH... rewrite Hsub with (c_x := c)... inversion Hst'.
 Qed.
 
 Global Hint Resolve mk_eq_under_base_is_type_closed: core.
@@ -155,15 +248,16 @@ Proof.
   setoid_rewrite H. auto.
 Qed.
 
-Lemma constant_eq_is_close: forall Gamma c, type_closed Gamma (mk_eq_constant c).
+Lemma constant_eq_is_close: forall Gamma c, type_closed_in_ctx Gamma (mk_eq_constant c).
 Proof.
   intros. constructor.
-  assert (type_closed_refinement nil (ty_of_const c) (fun (_ : state) (v : constant) => v = c)).
-  constructor.
-  unfold is_closed_refinement; destruct c; simpl; reflexivity.
-  apply type_closed_refinement_weakening with (Gamma1 := (erase_basetypectx (lcontxt_to_baseconctx Gamma))) (Gamma2 := nil); auto.
-  rewrite app_nil_r. auto.
-Qed.
+Admitted.
+(*   assert (closed_refinement_in_ctx nil (ty_of_const c) (fun (_ : state) (v : constant) => v = c)). *)
+(*   constructor. *)
+(*   unfold closed_refinement_under_state; destruct c; simpl; reflexivity. *)
+(*   apply closed_refinement_in_ctx_weakening with (Gamma1 := (erase_basetypectx (lcontxt_to_baseconctx Gamma))) (Gamma2 := nil); auto. *)
+(*   rewrite app_nil_r. auto. *)
+(* Qed. *)
 
 Global Hint Resolve mk_eq_constant_spec: core.
 Global Hint Resolve subst_constant_eq: core.
@@ -172,16 +266,22 @@ Global Hint Resolve constant_eq_is_close: core.
 (* type closed lemmas *)
 
 Lemma type_closed_add_post: forall (Gamma1 Gamma2: lcontxt) (tau: overunderty),
-    type_closed Gamma1 tau -> type_closed (Gamma1 ++ Gamma2) tau.
+    type_closed_in_ctx Gamma1 tau -> type_closed_in_ctx (Gamma1 ++ Gamma2) tau.
 Admitted.
 
 Lemma type_closed_add_pre: forall (Gamma1 Gamma2: lcontxt) (tau: overunderty),
-    type_closed Gamma2 tau -> type_closed (Gamma1 ++ Gamma2) tau.
+    type_closed_in_ctx Gamma2 tau -> type_closed_in_ctx (Gamma1 ++ Gamma2) tau.
+Admitted.
+
+Lemma st_type_closed_in_ctx_last_over_var: forall st Gamma x T phi, st (Gamma ++ ((x, Oty ({{v:T | phi}}))::nil)) (mk_eq_var T x).
+Admitted.
+
+Lemma st_type_closed_in_ctx_last_under_var: forall st Gamma x T phi, st (Gamma ++ ((x, Uty ([[v:T | phi]]))::nil)) (mk_eq_var T x).
 Admitted.
 
 Lemma type_closed_drop_post: forall (Gamma1 Gamma2: lcontxt) (tau: overunderty),
 	(forall x tau_x, l_find_right_most Gamma2 x = Some tau_x -> ~ appear_free_in_overunderty x tau) ->
-	type_closed (Gamma1 ++ Gamma2) tau -> type_closed Gamma1 tau.
+	type_closed_in_ctx (Gamma1 ++ Gamma2) tau -> type_closed_in_ctx Gamma1 tau.
 Admitted.
 
 Global Hint Resolve type_closed_add_pre: core.
@@ -197,33 +297,40 @@ Fixpoint erase_arr_bindings (Gamma: lcontxt): lcontxt :=
       end
   end.
 
-Lemma erase_arr_bindings_spec: forall (Gamma: lcontxt),
-    lcontxt_to_baseconctx Gamma = lcontxt_to_baseconctx (erase_arr_bindings Gamma).
-Proof.
-  intro Gamma. induction Gamma; auto.
-  destruct a as (x, xty).
-  destruct xty. destruct u; simpl; auto.
-  - rewrite IHGamma. auto.
-  - destruct o. simpl. rewrite IHGamma. auto.
-Qed.
+(* Lemma erase_arr_bindings_spec: forall (Gamma: lcontxt), *)
+(*     lcontxt_to_baseconctx Gamma = lcontxt_to_baseconctx (erase_arr_bindings Gamma). *)
+(* Proof. *)
+(*   intro Gamma. induction Gamma; auto. *)
+(*   destruct a as (x, xty). *)
+(*   destruct xty. destruct u; simpl; auto. *)
+(*   - rewrite IHGamma. auto. *)
+(*   - destruct o. simpl. rewrite IHGamma. auto. *)
+(* Qed. *)
 
 Lemma type_closed_even_without_arr_bindings: forall Gamma tau,
-    type_closed Gamma tau <-> type_closed (erase_arr_bindings Gamma) tau.
+    type_closed_in_ctx Gamma tau <-> type_closed_in_ctx (erase_arr_bindings Gamma) tau.
 Proof.
-  unfold type_closed. setoid_rewrite <- erase_arr_bindings_spec. reflexivity.
-Qed.
+Admitted.
+(*   unfold type_closed. setoid_rewrite <- erase_arr_bindings_spec. reflexivity. *)
+(* Qed. *)
 
-Definition lcontxt_to_basic_ctx (Gamma: lcontxt) := ncontxt_to_basic_ctx (erase_basetypectx (lcontxt_to_baseconctx Gamma)).
+(* Definition lcontxt_to_basic_ctx (Gamma: lcontxt) := ncontxt_to_basic_ctx (erase_basetypectx (lcontxt_to_baseconctx Gamma)). *)
 
-Global Hint Unfold lcontxt_to_basic_ctx: core.
+(* Global Hint Unfold lcontxt_to_basic_ctx: core. *)
 
 Inductive type_ctx_no_dup: lcontxt -> Prop :=
 | type_ctx_no_dup_nil: type_ctx_no_dup nil
 | type_ctx_no_dup_cons: forall x tau_x Gamma,
     l_find_right_most Gamma x = None ->
-    type_ctx_no_dup (Gamma <l> x :l: tau_x).
+    type_ctx_no_dup ((x, tau_x) :: Gamma).
 
 Global Hint Constructors type_ctx_no_dup: core.
+
+Lemma type_ctx_no_dup_cannot_find_last: forall Gamma b tau_b,
+    type_ctx_no_dup (Gamma ++ ((b, tau_b)::nil)) -> l_find_right_most Gamma b = None.
+Admitted.
+
+Global Hint Resolve type_ctx_no_dup_cannot_find_last: core.
 
 Lemma type_ctx_no_dup_fst_last_diff_name: forall a tau_a Gamma b tau_b,
     type_ctx_no_dup ((a, tau_a)::Gamma ++ ((b, tau_b)::nil)) -> a <> b.
@@ -237,35 +344,43 @@ Admitted.
 
 Global Hint Resolve type_ctx_no_dup_ctx_sub: core.
 
-(* type_closed_ctx: *)
+(* st_type_closed_ctx: *)
 (*   1. should also have no duplicate names *)
 (*   2. types are well_formed *)
 (*   3. types are closed *)
 
-Inductive type_closed_ctx: lcontxt -> Prop :=
-| type_closed_ctx_nil: type_closed_ctx nil
-| type_closed_ctx_cons: forall x tau_x Gamma,
+Inductive st_type_closed_ctx: nstate -> lcontxt -> Prop :=
+| st_type_closed_ctx_nil: forall st, st_type_closed_ctx st nil
+| st_type_closed_ctx_cons: forall st x tau_x Gamma,
     l_find_right_most Gamma x = None ->
-    type_closed_ctx Gamma ->
-    type_closed Gamma tau_x ->
+    st_type_closed_ctx st Gamma ->
+    st_type_closed_in_ctx st Gamma tau_x ->
     well_formed_type tau_x ->
-    type_closed_ctx (Gamma <l> x :l: tau_x).
+    st_type_closed_ctx st (Gamma <l> x :l: tau_x).
 
-Global Hint Constructors type_closed_ctx: core.
+Global Hint Constructors st_type_closed_ctx: core.
 
-Lemma type_closed_ctx_implies_type_ctx_no_dup: forall Gamma, type_closed_ctx Gamma -> type_ctx_no_dup Gamma.
+Lemma st_type_closed_ctx_emp_implies_all: forall st Gamma,
+    st_type_closed_ctx empty Gamma -> st_type_closed_ctx st Gamma.
 Admitted.
 
-Global Hint Resolve type_closed_ctx_implies_type_ctx_no_dup: core.
+Global Hint Resolve st_type_closed_ctx_emp_implies_all: core.
 
-Lemma type_closed_ctx_fst_last_diff_name: forall a tau_a Gamma b tau_b,
-    type_closed_ctx ((a, tau_a)::Gamma ++ ((b, tau_b)::nil)) -> a <> b.
+Lemma st_type_closed_ctx_implies_type_ctx_no_dup: forall st Gamma, st_type_closed_ctx st Gamma -> type_ctx_no_dup Gamma.
 Admitted.
 
-Lemma type_closed_ctx_prefix: forall Gamma1 Gamm2,
-    type_closed_ctx (Gamma1 ++ Gamm2) -> type_closed_ctx Gamma1.
+Global Hint Resolve st_type_closed_ctx_implies_type_ctx_no_dup: core.
+
+Lemma st_type_closed_ctx_fst_last_diff_name: forall st a tau_a Gamma b tau_b,
+    st_type_closed_ctx st ((a, tau_a)::Gamma ++ ((b, tau_b)::nil)) -> a <> b.
+Proof with eauto.
+  intros. eapply type_ctx_no_dup_fst_last_diff_name...
+Qed.
+
+Lemma st_type_closed_ctx_prefix: forall st Gamma1 Gamm2,
+    st_type_closed_ctx st (Gamma1 ++ Gamm2) -> st_type_closed_ctx st Gamma1.
 Admitted.
 
-Lemma type_closed_ctx_even_without_arr_bindings: forall Gamma,
-    type_closed_ctx Gamma -> type_closed_ctx (erase_arr_bindings Gamma).
-Admitted.
+(* Lemma st_type_closed_ctx_even_without_arr_bindings: forall st Gamma, *)
+(*     st_type_closed_ctx st Gamma -> st_type_closed_ctx (erase_arr_bindings Gamma). *)
+(* Admitted. *)
