proof/DenotationSpecsSimp.v
@@ -30,65 +30,195 @@ Lemma tmR_in_ctx_id_eq_c: forall st Gamma (id: string) c,
     (forall e tau, tmR_in_ctx_aux st Gamma tau e <-> tmR_in_ctx_aux st Gamma tau (subst id c e)).
 Admitted.
 
-Lemma tmR_in_ctx_state_implies_subst: forall (st: state) a (c_a: constant) Gamma tau,
-    st a = c_a ->
+Lemma tmR_in_ctx_state_implies_subst: forall (st: nstate) a (c_a: constant) Gamma tau,
+    st a = Some (tvalue c_a) ->
     l_find_right_most Gamma a = None ->
     (forall e, tmR_in_ctx_aux st Gamma tau e <-> tmR_in_ctx_aux st Gamma tau ([a := c_a] e)).
 Admitted.
 
+Lemma eta1: forall x1 x T e x2 (c_x:constant) x0,
+    x1<> x2 -> ~ x1 \FVtm c_x ->
+    (tlete x1 (vlam x T e) (tlete x2 c_x (tletapp x0 x1 x2 x0))) <=< (tlete x c_x e).
+Admitted.
 
 (* Assume there is no dup in the context to simplify the proof. *)
 Lemma tmR_in_ctx_preserve_oarr: forall Gamma st x (tau_x: overbasety) e (tau: underty),
-    type_ctx_no_dup (Gamma <l> x :l: Oty tau_x) ->
     tmR_in_ctx_aux st (Gamma <l> x :l: Oty tau_x) tau e ->
     tmR_in_ctx_aux st Gamma (x o: tau_x o--> tau) (vlam x (o\_ tau_x _/) e).
 Proof with eauto.
   intro Gamma.
-  induction Gamma; simpl; intros st x tau_x e tau Hctx HD.
+  induction Gamma; simpl; intros st x tau_x e tau HD.
   - setoid_rewrite app_nil_l in HD. inversion HD; subst. constructor... constructor... constructor...
     split.
-    + simpl. constructor... constructor... apply tmR_in_ctx_aux_implies_has_type in HD.
-      unfold lcontxt_to_basic_ctx in HD. unfold ncontxt_to_basic_ctx in HD. simpl in HD...
+    + simpl. constructor... constructor... apply tmR_in_ctx_aux_implies_has_type in HD...
     + intros c_x Hc_xD e3 Happ. inversion Happ; subst. simpl.
-      eapply step_preserve_under_denotation... eapply eta_reduction...
-      eapply step_preserve_under_denotation... eapply eta_application_const_to_lete_const...
-      assert (tmR_in_ctx_aux (x !-> c_x; st) [] tau (tlete x c_x e)) as HH... inversion HH; subst. inversion H0...
+      eapply step_preserve_under_denotation... apply eta1...
+      assert (tmR_in_ctx_aux (x |-> c_x; st) [] tau (tlete x c_x e)) as HH...
+      inversion HH; subst. inversion H1...
   - destruct a as (a & tau_a).
+    assert (type_ctx_no_dup ((a, tau_a) :: Gamma <l> x :l: tau_x)) as Hnodup...
     inversion HD; subst.
-    + constructor...
-      (* apply denotation_ctx_implies_last_well_formed_type in HD... inversion HD; subst. *)
+    + constructor... apply l_find_right_most_weak in H3. destruct H3...
       intros c_x Hc_xD.
       eapply step_preserve_ctx_denotation. apply eta_lete_const_to_subst.
-      simpl... destruct (eqb_spec a x)... exfalso. eapply type_ctx_no_dup_fst_last_diff_name...
+      simpl... destruct (eqb_spec a x)... { exfalso. eapply type_ctx_no_dup_fst_last_diff_name... }
       eapply step_preserve_ctx_denotation... apply eta_lete_const_to_subst_in_lam...
-      eapply IHGamma...
-      apply type_ctx_no_dup_ctx_sub with (Gamma1 := (a, Oty ({{v:T | phi}}))::nil)...
-    + constructor...
-      destruct H7 as (e_x_hat & He_x_hatD & HH).
+      (* eapply IHGamma... *)
+      (* apply type_ctx_no_dup_ctx_sub with (Gamma1 := (a, Oty ({{v:T | phi}}))::nil)... *)
+    + constructor... apply l_find_right_most_weak in H3. destruct H3...
+      destruct H9 as (e_x_hat & He_x_hatD & HH).
       exists e_x_hat. split...
-      intros e_x He_xD c_x Hc_xT Hc_xE.
+      intros e_x He_xD.
+      (* intros c_x Hc_xE Hc_xT e_x He_xD. *)
       eapply step_preserve_ctx_denotation... eapply eta_closed_term_can_captured_by_lam...
-      apply IHGamma...
-      apply type_ctx_no_dup_ctx_sub with (Gamma1 := (a, Uty ([[v:T | phi]]))::nil)...
-    + constructor...
+      (* apply IHGamma... *)
+      (* apply type_ctx_no_dup_ctx_sub with (Gamma1 := (a, Uty ([[v:T | phi]]))::nil)... *)
+    + constructor... apply l_find_right_most_weak in H3. destruct H3...
       intros e_x He_xD.
       eapply step_preserve_ctx_denotation... eapply eta_closed_term_can_captured_by_lam...
-      apply IHGamma...
-      apply type_ctx_no_dup_ctx_sub with (Gamma1 := (a, Uty tau_x0)::nil)...
+      (* apply IHGamma... *)
+      (* eapply type_ctx_no_dup_ctx_sub with (Gamma1 := (a, Uty (a0 o: {{v:T | phi}} o--> tau_b))::nil)... *)
+    + constructor... apply l_find_right_most_weak in H3. destruct H3...
+      intros e_x He_xD.
+      eapply step_preserve_ctx_denotation... eapply eta_closed_term_can_captured_by_lam...
+      (* apply IHGamma... *)
+      (* eapply type_ctx_no_dup_ctx_sub with (Gamma1 := (a, Uty (t1 u--> t2))::nil)... *)
 Qed.
 
+(* meet operation, the trick here is encode the conjunction into the target language, via a poly equal operator.
+
+  let x1 = e1 in
+  let x2 = e2 in
+  let x3 = x1 ==T x2 in
+  match x3 with
+  | true -> x2
+  | false -> err
+
+ *)
+Lemma meet_of_two_terms_exists: forall e1 e2 T,
+    empty |- e1 \Tin T -> empty |- e2 \Tin T -> (exists e3, (empty |- e3 \Tin T) /\ (forall c, e3 -->* c <-> e1 -->* c /\ e2 -->* c)).
+Admitted.
+
+Lemma meet_of_two_terms_implies_denotation: forall st tau e1 e2 e3,
+    under_tmR_aux st tau e1 -> under_tmR_aux st tau e2 ->
+    (forall c, e3 -->* c <-> e1 -->* c /\ e2 -->* c) -> under_tmR_aux st tau e3.
+Admitted.
+
+Global Hint Resolve meet_of_two_terms_implies_denotation: core.
+
+
+Lemma eta2: forall e2 (c2: constant) x1 e1 x2 x,
+    e2 -->* c2 ->
+    (tlete x1 e1 (tlete x2 c2 (tletapp x x1 x2 x))) <-< (tlete x1 e1 (tlete x2 e2 (tletapp x x1 x2 x))).
+Admitted.
+
+Lemma under_tmR_aux_st_update: forall x (c_x: constant) st tau,
+    (forall e, under_tmR_aux (x |-> (tvalue c_x); st) tau e <-> under_tmR_aux st (<u[ x |c-> c_x ]> tau) e).
+Admitted.
+
+ (* tmR_in_ctx_aux st ((a, {{v:T0 | phi0}}) :: Gamma) ([[v:T | phi]]) e2 *)
+
+
+Lemma eta3: forall x1 a (e_a: tm) Ta e1 x2 e2 x,
+    empty |- e_a \Tin Ta ->
+        (tlete a e_a (tlete x1 e1 (tlete x2 e2 (tletapp x x1 x2 x))))
+          <=< (tlete x1 (tlete a e_a e1) (tlete x2 (tlete a e_a e2) (tletapp x x1 x2 x))).
+Admitted.
+
+Global Hint Resolve tmR_has_type: core.
+
+Lemma tmR_in_ctx_preserve_application: forall Gamma st x1 x2 x (e1 e2: tm) tau a T phi,
+    x1 <> x2 -> ~ x1 \FVtm e2 ->
+    tmR_in_ctx_aux st Gamma (a o: {{v: T | phi}} o--> tau) e1 ->
+    tmR_in_ctx_aux st Gamma ([[v: T | phi]]) e2 ->
+    (forall (c2: constant), (forall e', tmR_in_ctx_aux st Gamma ([[v: T | phi]]) e' -> e' -->* c2) ->
+                       tmR_in_ctx_aux st Gamma (under_subst_c a c2 tau)
+                                      (tlete x1 e1 (tlete x2 e2 (tletapp x x1 x2 x)))
+    ).
+Proof with eauto.
+  intro Gamma.
+  induction Gamma; simpl; intros st x1 x2 x e1 e2 tau a0 T phi Hx1x2 Hx1free Hv1D Hv2D c2 Hc2Prop.
+  - assert (e2 -->* c2) as He2E...
+    inversion Hv1D; subst. inversion Hv2D; subst. clear Hv1D Hv2D.
+    inversion H; subst. inversion H0; subst. clear H H0.
+    (* inversion H0; subst. clear H0. *)
+    constructor... constructor...
+    inversion H3; subst. destruct H0 as (Hv1T & HH).
+    assert (under_tmR_aux (a0 |-> c2; st) tau (tlete x1 e1 (tlete x2 c2 (tletapp x x1 x2 x))))... apply HH... admit.
+    eapply step_preserve_under_denotation... apply eta2...
+    rewrite <- under_tmR_aux_st_update...
+  - destruct a as (a & tau_a).
+    assert (type_ctx_no_dup ((a, tau_a) :: Gamma)) as Hnodup...
+    inversion Hv1D; subst.
+    + constructor... inversion H3... inversion H5...
+      intros c_x He_xD. inversion Hv2D; subst.
+      assert (tmR_in_ctx_aux (a |-> c_x; st) Gamma (a0 o: {{v:T | phi}} o--> tau) (tlete a c_x e1)) as HHv1...
+      assert (tmR_in_ctx_aux (a |-> c_x; st) Gamma ([[v:T | phi]]) (tlete a c_x e2)) as HHv2...
+      assert (tmR_in_ctx_aux (a |-> c_x; st) Gamma (<u[ a0 |c-> c2 ]> tau) (tlete x1 (tlete a c_x e1) (tlete x2 (tlete a c_x e2) (tletapp x x1 x2 x)))). eapply IHGamma... admit.
+      eapply step_preserve_ctx_denotation... eapply eta3...
+    + constructor... inversion H3... inversion H5...
+      destruct H9 as (e_x_hat1 & He_x_hat1D & HH1).
+      inversion Hv2D; subst.
+      { destruct H14 as (e_x_hat2 & He_x_hat2D & HH2).
+        destruct (meet_of_two_terms_exists e_x_hat1 e_x_hat2 T0) as (e_x_hat3 & HT3 & HE3)...
+        - apply tmR_has_type in He_x_hat1D...
+        - apply tmR_has_type in He_x_hat2D...
+        - exists e_x_hat3... split... admit.
+          intros e_x He_xD.
+          assert (tmR_in_ctx_aux (a |-> e_x_hat1; st) Gamma (a0 o: {{v:T | phi}} o--> tau) (tlete a e_x e1)) as Hv1...
+          assert (tmR_in_ctx_aux (a |-> e_x_hat2; st) Gamma ([[v:T | phi]]) (tlete a e_x e2)) as Hv2...
+          assert (tmR_in_ctx_aux (a |-> e_x_hat3; st) Gamma (<u[ a0 |c-> c2 ]> tau)
+                                 (tlete x1 (tlete a e_x e1) (tlete x2 (tlete a e_x e2) (tletapp x x1 x2 x))))... eapply IHGamma... admit. admit. admit.
+          eapply step_preserve_ctx_denotation... eapply eta3...
+      }
+    + constructor... inversion H3... inversion H5...
+      inversion Hv1D; subst. inversion Hv2D; subst.
+      intros e_x He_xD.
+      assert (tmR_in_ctx_aux st Gamma (a0 o: {{v:T | phi}} o--> tau) (tlete a e_x e1)) as Hv1...
+      assert (tmR_in_ctx_aux st Gamma ([[v:T | phi]]) (tlete a e_x e2)) as Hv2...
+      assert (tmR_in_ctx_aux st Gamma (<u[ a0 |c-> c2 ]> tau) (tlete x1 (tlete a e_x e1) (tlete x2 (tlete a e_x e2) (tletapp x x1 x2 x))))... eapply IHGamma... admit.
+      eapply step_preserve_ctx_denotation... eapply eta3...
+    + constructor... inversion H3... inversion H5...
+      inversion Hv1D; subst. inversion Hv2D; subst.
+      intros e_x He_xD.
+      assert (tmR_in_ctx_aux st Gamma (a0 o: {{v:T | phi}} o--> tau) (tlete a e_x e1))...
+      assert (tmR_in_ctx_aux st Gamma ([[v:T | phi]]) (tlete a e_x e2))...
+      assert (tmR_in_ctx_aux st Gamma (<u[ a0 |c-> c2 ]> tau) (tlete x1 (tlete a e_x e1) (tlete x2 (tlete a e_x e2) (tletapp x x1 x2 x))))... eapply IHGamma... admit.
+      eapply step_preserve_ctx_denotation... eapply eta3...
+Admitted.
+
+
 Lemma tmR_in_ctx_preserve_arrarr: forall Gamma st x (tau_x: underty) e (tau: underty),
-    type_ctx_no_dup (Gamma <l> x :l: Uty tau_x) ->
     tmR_in_ctx_aux st (Gamma <l> x :l: Uty tau_x) tau e ->
     tmR_in_ctx_aux st Gamma (tau_x u--> tau) (vlam x (u\_ tau_x _/) e).
 Proof with eauto.
   intro Gamma.
-  induction Gamma; simpl; intros st x tau_x e tau Hctx HD.
-  - setoid_rewrite app_nil_l in HD. setoid_rewrite app_nil_l in Hctx.
+  induction Gamma; simpl; intros st x tau_x e tau HD.
+  - setoid_rewrite app_nil_l in HD.
 Admitted.
 
+(* Lemma eta_closed_term_can_penetrate_letapp: forall a e_a Ta x v1 v2 y Ty, *)
+(*     empty |- e_a \Tin Ta -> *)
+(*             a <> y -> ~ y \FVtm e_a -> *)
+(*             (tletapp x (vlam y Ty (tlete a e_a (tletapp x v1 y x))) v2 x) *)
+(*               <=< (tlete a e_a (tletapp x v1 v2 x)). *)
+(* Admitted. *)
+
+(* Another version of the denotation definition; HACK: how to prove it?  *)
+(* Lemma e_x_hat_exists: forall st (T: base_ty) (phi: refinement), *)
+(*     exists e_x_hat, *)
+(*       under_tmR_aux st ([[v:T | phi]]) e_x_hat /\ *)
+(*       (forall (c_x : constant), empty |- c_x \Vin T -> (e_x_hat -->* c_x <-> phi st c_x)). *)
+(* Admitted. *)
+
+(* Lemma e_x_hat_minimal: forall st (T: base_ty) (phi: refinement) e_x_hat e_x, *)
+(*     under_tmR_aux st ([[v:T | phi]]) e_x_hat -> *)
+(*     under_tmR_aux st ([[v:T | phi]]) e_x -> *)
+(*     (forall (c_x : constant), empty |- c_x \Vin T -> (e_x_hat -->* c_x <-> phi st c_x)) -> *)
+(*     e_x_hat <-< e_x. *)
+(* Admitted. *)
+
 Lemma tmR_in_ctx_preserve_arrarr_application: forall Gamma st x (v1 v2: value) tau tau1,
-    (* ctx_inv Gamma -> *)
     tmR_in_ctx_aux st Gamma (tau1 u--> tau) v1 ->
     tmR_in_ctx_aux st Gamma tau1 v2 ->
     tmR_in_ctx_aux st Gamma tau (tletapp x v1 v2 x).
@@ -100,41 +230,79 @@ Proof with eauto.
     eapply HH with (e3:=e3) in H4... constructor... eapply step_preserve_under_denotation... destruct He3E...
   - destruct a as (a & tau_a).
     inversion Hv1D; subst.
-    + constructor... { inversion H3; subst... } inversion Hv2D; subst.
+    + constructor... { inversion H5; subst... } inversion Hv2D; subst.
       intros c_x He_xD.
       (* make HHv1 and HHv2 to value. *)
-      assert (tmR_in_ctx_aux (a !-> c_x; st) Gamma (tau_x u--> tau) ([a := c_x] v1)) as HHv1...
-      { eapply step_preserve_ctx_denotation... apply eta_lete_const_to_subst. } clear H7.
-      assert (tmR_in_ctx_aux (a !-> c_x; st) Gamma tau_x ([a := c_x] v2)) as HHv2...
-      { eapply step_preserve_ctx_denotation... apply eta_lete_const_to_subst. } clear H11.
+      assert (tmR_in_ctx_aux (a |-> c_x; st) Gamma (tau_x u--> tau) ([a := c_x] v1)) as HHv1...
+      { eapply step_preserve_ctx_denotation... apply eta_lete_const_to_subst. }
+      assert (tmR_in_ctx_aux (a |-> c_x; st) Gamma tau_x ([a := c_x] v2)) as HHv2...
+      { eapply step_preserve_ctx_denotation... apply eta_lete_const_to_subst. }
       eapply step_preserve_ctx_denotation. apply eta_lete_const_to_subst. rewrite subst_letapp_penetrate.
       eapply IHGamma...
-    + constructor... { inversion H3; subst... }
-      destruct H7 as (e_x_hat & He_x_hatD & HH).
+    + constructor... { inversion H5; subst... }
+      destruct H9 as (e_x_hat & He_x_hatD & HH).
       exists e_x_hat. split...
-      intros e_x He_xD c_x Hc_xT Hc_xE.
-      (* (need context inv) *)
+      (* intros c_x Hc_xT Hc_xD e_x He_xD. *)
+      (* assert (tmR_in_ctx_aux (a |-> c_x; st) Gamma (tau_x u--> tau) (tlete a e_x v1))... *)
+      (* inversion Hv2D; subst... *)
+      (* destruct v2. admit. destruct c. admit. *)
 Admitted.
+
+Lemma eta4: forall x1 (v1: value) x2 (c2: constant) x,
+    x1 <> x2 ->
+      tlete x1 v1 (tlete x2 c2 (tletapp x x1 x2 x)) <-< tletapp x v1 c2 x.
+Admitted.
+
 
 Lemma tmR_in_ctx_preserve_oarr_c_application: forall Gamma st x (v1: value) (c2: constant) tau a T phi,
     tmR_in_ctx_aux st Gamma (a o: {{v: T | phi}} o--> tau) v1 ->
     tmR_in_ctx_aux st Gamma ([[v: T | phi]]) c2 ->
     tmR_in_ctx_aux st Gamma (under_subst_c a c2 tau) (tletapp x v1 c2 x).
+Proof with eauto.
+  intro Gamma; simpl; intros st x v1 c2 tau a0 T phi Hv1D Hv2D.
+  destruct (exists_fresh_var_of_value c2) as (x1 & x2 & Hx1x2 & Hfree).
+  eapply tmR_in_ctx_preserve_application with (x1:=x1) (x2:=x2) (x:=x) (e2:=c2) (c2:=c2) in Hv1D...
+  eapply step_preserve_ctx_denotation... eapply eta4... admit.
 Admitted.
 
 Lemma tmR_in_ctx_preserve_oarr_var_application: forall Gamma st x (v1: value) (name2: string) tau a T phi,
     tmR_in_ctx_aux st Gamma (a o: {{v: T | phi}} o--> tau) v1 ->
     tmR_in_ctx_aux st Gamma ([[v: T | phi]]) name2 ->
     tmR_in_ctx_aux st Gamma (under_subst_id a name2 tau) (tletapp x v1 name2 x).
+Proof with eauto.
+  intro Gamma; simpl; intros st x v1 c2 tau a0 T phi Hv1D Hv2D.
+  destruct (exists_fresh_var_of_value c2) as (x1 & x2 & Hx1x2 & Hfree).
 Admitted.
+(*   intro Gamma. *)
+(*   induction Gamma; simpl; intros st x v1 c2 tau a0 T phi Hv1D Hv2D. *)
+(*   - admit. *)
+(*   - destruct a as (a & tau_a). *)
+(*     inversion Hv1D; subst. *)
+(*     + constructor... admit. admit. *)
+(*     + constructor... admit. *)
+(*       destruct H7 as (e_x_hat & He_x_hatD & HH). *)
+(*       assert (forall c_x : constant, *)
+(*                  phi st c_x -> *)
+(*                  empty |- c_x \Vin T0 -> *)
+(*                          forall e_x : tm, *)
+(*                            under_tmR_aux st ([[v:T0 | phi0]]) e_x -> *)
+(*                            tmR_in_ctx_aux (a |-> c_x; st) Gamma (a0 o: {{v:T | phi}} o--> tau) (tlete a e_x v1)). *)
+(*       { intros... apply HH... admit. } clear HH. clear He_x_hatD e_x_hat. *)
+(*       inversion Hv2D; subst. *)
+(*       destruct H11 as (e_x_hat & He_x_hatD & HH). *)
+(*       exists e_x_hat. split... *)
+(*       intros c_x Hc_xD Hc_xT e_x He_xD. *)
+(*       assert (tmR_in_ctx_aux (a |-> c_x; st) Gamma ([[v:T | phi]]) (tlete a e_x c2))... clear HH. *)
+(* Admitted. *)
 
 Lemma tmR_in_ctx_preserve_matchb_true: forall Gamma st (v: value) e1 e2 tau,
+    type_ctx_no_dup Gamma ->
     tmR_in_ctx_aux st Gamma (mk_eq_constant true) v ->
     tmR_in_ctx_aux st Gamma tau e1 ->
     tmR_in_ctx_aux st Gamma tau (tmatchb v e1 e2).
 Proof with eauto.
-  intros Gamma st v e1 e2 tau Hv He1.
-  assert ((exists n : bool, v = n) \/ (exists name : string, v = name)) as HH. apply tmR_in_ctx_aux_implies_has_type in Hv. inversion Hv; subst. apply bool_value_cid_exists in H1...
+  intros Gamma st v e1 e2 tau Hnodup Hv He1.
+  assert ((exists n : bool, v = n) \/ (exists name : string, v = name)) as HH. apply tmR_in_ctx_aux_implies_has_type in Hv... inversion Hv; subst. apply bool_value_cid_exists in H1...
   destruct HH.
   - destruct H as (b & Hb); subst. apply mk_eq_constant_is_itsefl_in_ctx in Hv. rewrite Hv.
     eapply step_preserve_ctx_denotation... apply eta_matchb_true...
@@ -145,12 +313,13 @@ Qed.
 
 
 Lemma tmR_in_ctx_preserve_matchb_false: forall st Gamma (v: value) e1 e2 tau,
+    type_ctx_no_dup Gamma ->
     tmR_in_ctx_aux st Gamma (mk_eq_constant false) v ->
     tmR_in_ctx_aux st Gamma tau e2 ->
     tmR_in_ctx_aux st Gamma tau (tmatchb v e1 e2).
 Proof with eauto.
-  intros st Gamma v e1 e2 tau Hv He1.
-  assert ((exists n : bool, v = n) \/ (exists name : string, v = name)) as HH. apply tmR_in_ctx_aux_implies_has_type in Hv. inversion Hv; subst. apply bool_value_cid_exists in H1...
+  intros st Gamma v e1 e2 tau Hnodup Hv He1.
+  assert ((exists n : bool, v = n) \/ (exists name : string, v = name)) as HH. apply tmR_in_ctx_aux_implies_has_type in Hv... inversion Hv; subst. apply bool_value_cid_exists in H1...
   destruct HH.
   - destruct H as (b & Hb); subst. apply mk_eq_constant_is_itsefl_in_ctx in Hv. rewrite Hv.
     eapply step_preserve_ctx_denotation... apply eta_matchb_false...
