proof/WellFormedSpecsSimp.v
@@ -1,0 +1,106 @@
+Set Warnings "-notation-overridden,-parsing".
+From PLF Require Import Maps.
+From PLF Require Import CoreLangSimp.
+From PLF Require Import NormalTypeSystemSimp.
+From PLF Require Import LinearContext.
+From PLF Require Import RfTypeDef.
+From PLF Require Import TypeClosedSimp.
+From PLF Require Import DenotationSimp.
+From PLF Require Import WellFormedSimp.
+From PLF Require Import DenotationSpecsSimp.
+From Coq Require Import Logic.FunctionalExtensionality.
+From Coq Require Import Logic.ClassicalFacts.
+From Coq Require Import Lists.List.
+
+Import CoreLangSimp.
+Import LinearContext.
+Import TypeClosedSimp.
+Import DenotationSimp.
+Import WellFormedSimp.
+Import DenotationSpecsSimp.
+Import ListNotations.
+
+Lemma tmR_nst_no_free_implies_eq: forall st x e_x_hat (tau: underty),
+    ~ appear_free_in_underty x tau -> (forall e, tmR_aux (x |-> e_x_hat; st) tau e <-> tmR_aux st tau e).
+Admitted.
+
+Global Hint Rewrite tmR_nst_no_free_implies_eq: core.
+Global Hint Resolve tmR_has_type: core.
+
+Lemma lete_ctx_inv_implies_safe_dropping_1_to_1: forall Gamma st x tau_x tau,
+    ~ appear_free_in_underty x tau ->
+    ctx_inv st (Gamma ++ ((x, Uty tau_x)::nil)) ->
+    (forall e, tmR_in_ctx_aux st (Gamma ++ ((x, Uty tau_x)::nil)) tau e ->
+          (forall e_x, tmR_in_ctx_aux st Gamma tau_x e_x -> tmR_in_ctx_aux st Gamma tau (tlete x e_x e))).
+Proof with eauto.
+  intro Gamma. induction Gamma; simpl; intros st x tau_x tau Hfree Hinv e HeD e_x He_xD.
+  - constructor... inversion He_xD; subst. inversion HeD; subst.
+    + destruct H10 as (e_x_hat & He_x_hatD & HH).
+      assert (tmR_in_ctx_aux (x |-> e_x_hat; st) [] tau (tlete x e_x e)) as HD... inversion HD; subst...
+      rewrite <- tmR_nst_no_free_implies_eq...
+    + assert (tmR_in_ctx_aux st [] tau (tlete x e_x e)) as HD... inversion HD; subst...
+    + assert (tmR_in_ctx_aux st [] tau (tlete x e_x e)) as HD... inversion HD; subst...
+  - destruct a as (a & tau_a).
+    inversion HeD; subst.
+    + constructor... admit.
+      intros c_x Hc_xD.
+      assert (tmR_in_ctx_aux (a |-> c_x; st) (Gamma ++ ((x, Uty tau_x)::nil)) tau (tlete a c_x e))...
+      inversion He_xD; subst...
+      assert (tmR_in_ctx_aux (a |-> c_x; st) Gamma tau_x (tlete a c_x e_x))...
+      assert (tmR_in_ctx_aux (a |-> c_x; st) Gamma tau (tlete x e_x (tlete a c_x e))). eapply IHGamma... admit.
+      admit.
+    + constructor... admit.
+      destruct H9 as (e_x_hat1 & He_x_hatD1 & HH1).
+      inversion He_xD; subst...
+      destruct H14 as (e_x_hat2 & He_x_hatD2 & HH2).
+      destruct (meet_of_two_terms_exists e_x_hat1 e_x_hat2 T) as (e_x_hat3 & HT3 & HE3)... apply tmR_has_type in He_x_hatD1... apply tmR_has_type in He_x_hatD2...
+      exists e_x_hat3. split... admit.
+      intros e_x' He_xD'.
+      assert (tmR_in_ctx_aux (a |-> e_x_hat1; st) (Gamma ++ ((x, Uty tau_x)::nil)) tau (tlete a e_x' e)). apply HH1...
+      assert (tmR_in_ctx_aux (a |-> e_x_hat2; st) Gamma tau_x (tlete a e_x' e_x)). apply HH2...
+      assert (tmR_in_ctx_aux (a |-> e_x_hat3; st) Gamma tau (tlete x (tlete a e_x' e_x) (tlete a e_x' e)))... eapply IHGamma with (tau_x:= tau_x)... admit. admit. admit. admit.
+    + constructor... admit.
+      inversion He_xD; subst.
+      intros e_x' He_xD'.
+      assert (tmR_in_ctx_aux st (Gamma ++ ((x, Uty tau_x)::nil)) tau (tlete a e_x' e))...
+      assert (tmR_in_ctx_aux st Gamma tau_x (tlete a e_x' e_x))...
+      assert (tmR_in_ctx_aux st Gamma tau (tlete x (tlete a e_x' e_x) (tlete a e_x' e)))... eapply IHGamma... admit.
+      admit.
+    + constructor... admit.
+      inversion He_xD; subst.
+      intros e_x' He_xD'.
+      assert (tmR_in_ctx_aux st (Gamma ++ ((x, Uty tau_x)::nil)) tau (tlete a e_x' e))...
+      assert (tmR_in_ctx_aux st Gamma tau_x (tlete a e_x' e_x))...
+      assert (tmR_in_ctx_aux st Gamma tau (tlete x (tlete a e_x' e_x) (tlete a e_x' e)))... eapply IHGamma... admit.
+      admit.
+Admitted.
+
+
+
+
+Lemma tletbiop_ctx_inv_implies_safe_dropping_1_to_1: forall Gamma x tau,
+    (forall e op (v1 v2: cid),
+        ctx_inv empty (Gamma ++ ((x, Uty (mk_op_retty_from_cids op v1 v2))::nil)) ->
+        tmR_in_ctx_all_st (Gamma ++ ((x, Uty (mk_op_retty_from_cids op v1 v2))::nil)) tau e ->
+        tmR_in_ctx_all_st (Gamma <l> x :l: ((mk_op_retty_from_cids op v1 v2))) tau e ->
+        tmR_in_ctx_all_st Gamma tau (tletbiop x op v1 v2 e)).
+Admitted.
+
+Lemma tletapp_oarr_ctx_inv_implies_safe_dropping_1_to_1: forall Gamma x tau_x tau,
+    (forall e (v1: value) (v2: cid) a T phi1,
+        tmR_in_ctx_all_st Gamma (a o: {{v: T | phi1}} o--> tau_x) v1 ->
+        tmR_in_ctx_all_st Gamma ([[v: T | phi1]]) v2 ->
+        ctx_inv empty (Gamma ++ ((x, Uty (under_subst_cid a v2 tau_x))::nil)) ->
+        tmR_in_ctx_all_st (Gamma ++ ((x, Uty (under_subst_cid a v2 tau_x))::nil)) tau e ->
+        tmR_in_ctx_all_st Gamma tau (tletapp x v1 v2 e)).
+Admitted.
+
+Lemma tletapp_arrarr_ctx_inv_implies_safe_dropping_1_to_1: forall Gamma x tau_x tau,
+    ~ appear_free_in_underty x tau_x ->
+    ctx_inv empty (Gamma ++ ((x, Uty tau_x)::nil)) ->
+    (forall e, tmR_in_ctx_all_st (Gamma ++ ((x, Uty tau_x)::nil)) tau e ->
+          (forall (v1 v2: value) t1,
+              tmR_in_ctx_all_st Gamma (t1 u--> tau_x) v1 ->
+              tmR_in_ctx_all_st Gamma t1 v2 ->
+              tmR_in_ctx_all_st Gamma tau (tletapp x v1 v2 e))).
+Admitted.
